\section{Combination}

\subsection{Combination Identities}
\begin{equation}
{{n}\choose{r}} = \frac{n!}{r!(n-r)!}
\end{equation}

\subsection{Mirror Identity}
\begin{equation}
{{n}\choose{r}} = {{n}\choose{n-r}}
\end{equation}

\subsection{Pascal's Triangle Identity}
\begin{equation}
{{n}\choose{r}} = {{n-1}\choose{r-1}} + {{n-1}\choose{r}}
\end{equation}

\subsection{Extended Pascal's Triangle Identity}
\begin{equation}
{{n}\choose{r}} = \sum \limits_{i=0}^k{{{n-k}\choose{r-k-i}}{{k}\choose{i}}}
\end{equation}

\subsection{Row Sums}
\begin{equation}
\sum \limits_{j=0}^n{{n}\choose{j}} = 2^n
\end{equation}

\subsection{Diagonal Sums}
\begin{equation}
\sum \limits_{i=r}^n{{i}\choose{r}} = {{n+1}\choose{r+1}}
\end{equation}

\subsection{Second Order Diagonal Sum}
\begin{equation}
\sum \limits_{i=r}^n{(n-i+1){{i}\choose{r}}} = {{n+2}\choose{r+2}}
\end{equation}

\subsection{kth Order Diagonal Sum}
\begin{equation}
\sum \limits_{i=r}^n{{{n-i+k-1}\choose{k-1}}{{i}\choose{r}}} = {{n+k}\choose{r+k}}
\end{equation}
